\documentclass{article}
\usepackage[english]{babel}
\usepackage[a4paper,top=2cm,bottom=2cm,left=3cm,right=3cm,marginparwidth=1.75cm]{geometry}
% Useful packages
\usepackage{amsmath}
\usepackage{graphicx}
\usepackage{subcaption}
\usepackage[colorlinks=true, allcolors=black]{hyperref}
\usepackage{pdfpages}
\usepackage{float}%图片包
%\usepackage{cite}
\usepackage[backend=bibtex]{biblatex}
%more math symbols
\usepackage{amssymb}

\title{Analyse First order or Crossover}
\author{Xin-Peng Li}
%Start of the document
\begin{document}
\maketitle
When $\mu'\leq R_B$, the equation only have one solution, hence the multisolution zone must be $\mu'>R_B$. (There exists one possibility that both in $\mu'\leq R_B$ and $\mu'>R_B$ has at least one solution, but this case will not happen in CEP, so we ignore)
When $\mu'>R_B$, the equation becomes
\begin{equation}
    \begin{split}
    R_B=&m+\frac{8}{3\pi}\frac{\alpha_{IR}}{m_G^2}\int_{\mu'^2-R_B^2}^{\Lambda^2}\frac{R_Bs^{\frac{1}{2}}}{\sqrt{s+R_B^2}}ds\\
        =&m+\frac{8}{3\pi}\frac{\alpha_{IR}R_B}{m_G^2}\left[R_B^2\ln(\sqrt{x+R_B^2}-\sqrt{x})+\sqrt{x(x+R_B^2)}\right]|_{\mu'^2-R_B^2}^{\Lambda^2}\\
        =&m+\frac{8}{3\pi}\frac{\alpha_{IR}R_B}{m_G^2}\left[R_B^2\ln\frac{\sqrt{\Lambda^2+R_B^2}-\Lambda}{\mu'-\sqrt{\mu'^2-R_B^2}}+\Lambda\sqrt{\Lambda^2+R_B^2}-\mu'\sqrt{\mu'^2-R_B^2}\right]
    \end{split}
\end{equation}
When the first order transition happens, we will get the picture as below:
\begin{figure}[H]
    \centering
    \includegraphics[width=0.8\textwidth]{pic/shili.pdf}
    \caption{There exists two points $(\mu_1,R_{B1}),(\mu_2,R_{B2})$; If the transition is crossover, we could not get these two points.}
\end{figure}
Define $\frac{8}{3\pi}\frac{\alpha_{IR}}{m_G^2}=k$. At these two points, the following relationship must be satisfied:
\begin{itemize}
    \item 
    \begin{equation}
        \begin{split}
            F(x)=m+kx\left[x^2\ln\frac{\sqrt{\Lambda^2+x^2}-\Lambda}{\mu'-\sqrt{\mu'^2-x^2}}+\Lambda\sqrt{\Lambda^2+x^2}-\mu'\sqrt{\mu'^2-x^2}\right]-x=0
        \end{split}
    \end{equation}
    \item 
    \begin{equation}\label{F'}
        \begin{split}
            F'(x)=\frac{k\Lambda(3x^2+\Lambda^2)}{\sqrt{x^2+\Lambda^2}}-k\mu'\sqrt{\mu'^2-x^2}+3kx^2\ln\frac{\sqrt{\Lambda^2+x^2}-\Lambda}{\mu'-\sqrt{\mu'^2-x^2}}-1=0
        \end{split}
    \end{equation}
\end{itemize}
Solve the simultaneous equations and eliminate the logarithm part, we could get
\begin{equation}
    \begin{split}
        &\frac{3}{2}m-kx\mu'\sqrt{\mu'^2-x^2}-x+\frac{kx\Lambda^3}{\sqrt{\Lambda^2+x^2}}=0\\
        &\Leftrightarrow \mu'\sqrt{\mu'^2-x^2}=\frac{3}{2}\frac{m}{kx}-\frac{1}{k}+\frac{\Lambda^3}{\sqrt{\Lambda^2+x^2}}\equiv \frac{t(x)}{2}\\
        &\Leftrightarrow \mu'=\sqrt{\frac{x^2+\sqrt{x^4+t^2(x)}}{2}}
    \end{split}
\end{equation}
where $t(x)=\frac{3m}{kx}-\frac{2}{k}+\frac{2\Lambda^3}{\sqrt{\Lambda^2+x^2}}$
Substitute this equation into \eqref{F'}, we could get
    \begin{equation}
        \begin{split}
        &\frac{kx^2\Lambda}{\sqrt{x^2+\Lambda^2}}-\frac{1}{2}\frac{m}{x}+kx^2\ln\frac{\sqrt{\Lambda^2+x^2}-\Lambda}{\mu'-\sqrt{\mu'^2-x^2}}=0\\
        &\Leftrightarrow \frac{kx^2\Lambda}{\sqrt{x^2+\Lambda^2}}-\frac{1}{2}\frac{m}{x}+kx^2\ln\frac{\sqrt{\Lambda^2+x^2}-\Lambda}{(\sqrt{x^4+t^2}-t)^{\frac{1}{2}}}=0\\
        &\Leftrightarrow \frac{\Lambda}{\sqrt{x^2+\Lambda^2}}-\frac{1}{2}\frac{m}{kx^3}+\ln(\sqrt{\Lambda^2+x^2}-\Lambda)-\frac{1}{2}\ln(\sqrt{x^4+t^2}-t)\\
        &= \frac{\Lambda}{\sqrt{x^2+\Lambda^2}}-\frac{1}{2}\frac{m}{kx^3}+\ln\frac{\sqrt{\Lambda^2+x^2}-\Lambda}{(\sqrt{x^4+t^2}-t)^{\frac{1}{2}}}=0\equiv F(x)
        \end{split}
    \end{equation}
    If first order transition, the equation above must have two solutions; if crossover, the equation do not have any solution (in $x<M_0$).\\
    So the CEP is:
    \begin{itemize}
        \item \begin{equation}\label{1}
            F(x)=\frac{\Lambda}{\sqrt{x^2+\Lambda^2}}-\frac{1}{2}\frac{m}{kx^3}+\ln\frac{\sqrt{\Lambda^2+x^2}-\Lambda}{(\sqrt{x^4+t^2}-t)^{\frac{1}{2}}}= 0
        \end{equation}
        \item \begin{equation}\label{2}
            xF'(x)=\frac{3m}{2kx^3}+\frac{xt'}{2\sqrt{x^4+t^2}}+\frac{\Lambda^3}{(x^2+\Lambda^2)^{\frac{3}{2}}}-\frac{t}{\sqrt{x^4+t^2}}=0
        \end{equation}
        where $t'=\frac{dt}{dx}=-\frac{3m}{kx^2}-\frac{2x\Lambda^3}{(x^2+\Lambda^2)^{\frac{3}{2}}}$.
    \end{itemize}
    We have use a fact that if $F(x)=0, F'(x)=0$, then $x^nF(x)=0, x^nF'(x)=0$.\\
Solve the \autoref{2}, we could get
\begin{equation}
        \frac{3m}{2kx^3}+\frac{1}{\sqrt{x^4+t^2}}(\frac{xt'}{2}-t)+\frac{\Lambda^3}{(x^2+\Lambda^2)^\frac{3}{2}}= 0
\end{equation}
This equation is not a simple equation, we could numerically get a solution $x_0=x(m,k,\Lambda)$, and take into \autoref{1}. If $F(x_0)>0$, first order transition; If $F(x_0)\leq 0$, crossover.\\
% 这个分析 没有考虑C的影响
\end{document}

